Prove decomp_eq with admitted lemmas

B_Unification/sve.v
@@ -17,20 +17,63 @@ Fixpoint get_var (p : poly) : option var :=
 
 Definition has_var (x : var) := existsb (beq_nat x).
 
-Definition elim_var (x : var) (p : poly) : pair poly :=
-  partition (has_var x) p.
+Definition elim_var (x : var) (p : poly) : poly :=
+  map (remove var_eq_dec x) p.
+
+Definition div_by_var (x : var) (p : poly) : pair poly :=
+  let (qx, r) := partition (has_var x) p in
+  (elim_var x qx, r).
 
 Definition decomp (p : poly) : option (prod var (pair poly)) :=
   match get_var p with
   | None => None
-  | Some x => Some (x, (elim_var x p))
+  | Some x => Some (x, (div_by_var x p))
   end.
 
+Lemma elim_var_mul : forall x p q,
+  (forall m, In m p -> In x m) ->
+  elim_var x p = q ->
+  p = mulMP [x] q.
+Proof.
+Admitted.
+
+Lemma part_fst_true : forall X p (x t f : list X),
+  partition p x = (t, f) ->
+  (forall a, In a t -> p a = true).
+Proof.
+Admitted.
+
+Lemma has_var_eq_in : forall x m,
+  has_var x m = true <-> In x m.
+Proof.
+Admitted.
+
 Lemma decomp_eq : forall x p q r,
+  is_poly p ->
   decomp p = Some (x, (q, r)) ->
   p = addPP (mulMP [x] q) r.
 Proof.
-Admitted.
+  intros x p q r HP HD.
+  assert (HE: div_by_var x p = (q, r)).
+  unfold decomp in HD. destruct (get_var p); inversion HD; auto.
+  
+  unfold div_by_var in HE.
+  destruct ((partition (has_var x) p)) as [qx r0] eqn:Hqr.
+  injection HE. intros Hr Hq.
+
+  assert (HIH: forall m, In m qx -> In x m). intros.
+  apply has_var_eq_in.
+  apply (part_fst_true _ _ _ _ _ Hqr _ H).
+  apply (elim_var_mul _ _ _ HIH) in Hq.
+  
+  unfold is_poly in HP.
+  destruct HP as [Hnd].
+  apply (set_part_add (has_var x) _ _ _ Hnd).
+  rewrite <- Hq.
+  rewrite <- Hr.
+  apply Hqr.
+Qed.
+
 
 Definition build_poly (q r : poly) : poly := 
   mulPP (addPP [[]] q) r.
@@ -51,7 +94,7 @@ Lemma decomp_unif : forall x p q r s,
 Proof.
   unfold build_poly, unifier.
   intros x p q r s HPp HD Hsp0.
-  apply decomp_eq in HD as Hp.
+  apply (decomp_eq _ _ _ _ HPp) in HD as Hp.
   (* multiply both sides of Hsp0 by s(q+1) *)
   assert (exists q1, q1 = addPP [[]] q) as [q1 Hq1]. eauto.
   assert (exists sp, sp = substP s p) as [sp Hsp]. eauto.
